Add `LContext` and operators to typing rules (#203)
Makes `HasType` consistent with behavior of the typechecker by adding
`LContext` and rules for operators. In particular, this PR adds the
condition that constants are well-typed only if their corresoponding
type is known and adds rules for annotated and un-annotated operators
based on their `Factory` instance. It also adds a rule for annotated
free variables. Annotated operators and free variables are somewhat
complex, as they require the annotation to be an instantiation of their
general type.

By submitting this pull request, I confirm that you can use, modify,
copy, and redistribute this contribution, under the terms of your
choice.

---------

Co-authored-by: Josh Cohen <cohenjo@amazon.com>
Co-authored-by: Shilpi Goel <shigoel@gmail.com>

Strata/DL/Lambda/LExprTypeSpec.lean
@@ -50,85 +50,121 @@ def LTy.open (x : TyIdentifier) (xty : LMonoTy) (ty : LTy) : LTy :=
       ty
 
 /--
-Typing relation for `LExpr`s.
-
-(TODO) Add the introduction and elimination rules for `.tcons`.
+Open `ty` by instantiating all its bound variables with `tys`, giving the
+`LMonoTy` that results. `tys` should have length equal to the number of bound
+variables in `ty`.
 -/
-inductive HasType {IDMeta : Type} [DecidableEq IDMeta]:
+def LTy.openFull (ty: LTy) (tys: List LMonoTy) : LMonoTy :=
+  LMonoTy.subst [(List.zip (LTy.boundVars ty) tys)] (LTy.toMonoTypeUnsafe ty)
+
+/--
+Typing relation for `LExpr`s.
+-/
+inductive HasType {IDMeta : Type} [DecidableEq IDMeta] (C: LContext IDMeta):
   (TContext IDMeta) → (LExpr LMonoTy IDMeta) → LTy → Prop where
-  | tmdata : ∀ Γ info e ty, HasType Γ e ty →
-                            HasType Γ (.mdata info e) ty
+  | tmdata : ∀ Γ info e ty, HasType C Γ e ty →
+                            HasType C Γ (.mdata info e) ty
 
   | tbool_const : ∀ Γ b,
-            HasType Γ (.boolConst b) (.forAll [] .bool)
+            C.knownTypes.containsName "bool" →
+            HasType C Γ (.boolConst b) (.forAll [] .bool)
   | tint_const : ∀ Γ n,
-            HasType Γ (.intConst n) (.forAll [] .int)
+            C.knownTypes.containsName "int" →
+            HasType C Γ (.intConst n) (.forAll [] .int)
   | treal_const : ∀ Γ r,
-            HasType Γ (.realConst r) (.forAll [] .real)
+            C.knownTypes.containsName "real" →
+            HasType C Γ (.realConst r) (.forAll [] .real)
   | tstr_const : ∀ Γ s,
-            HasType Γ (.strConst s) (.forAll [] .string)
+            C.knownTypes.containsName "string" →
+            HasType C Γ (.strConst s) (.forAll [] .string)
   | tbitvec_const : ∀ Γ n b,
-            HasType Γ (.bitvecConst n b) (.forAll [] (.bitvec n))
+            C.knownTypes.containsName "bitvec" →
+            HasType C Γ (.bitvecConst n b) (.forAll [] (.bitvec n))
 
-  | tvar : ∀ Γ x ty, Γ.types.find? x = some ty → HasType Γ (.fvar x none) ty
+  | tvar : ∀ Γ x ty, Γ.types.find? x = some ty → HasType C Γ (.fvar x none) ty
+
+  /-
+  For an annotated free variable (or operator, see `top_annotated`), it must be
+  the case that the claimed type `ty_s` is an instantiation of the general type
+  `ty_o`. It suffices to show the existence of a list `tys` that, when
+  substituted for the bound variables in `ty_o`, results in `ty_s`.
+  -/
+  | tvar_annotated : ∀ Γ x ty_o ty_s tys,
+            Γ.types.find? x = some ty_o →
+            tys.length = ty_o.boundVars.length →
+            LTy.openFull ty_o tys = ty_s →
+            HasType C Γ (.fvar x (some ty_s)) (.forAll [] ty_s)
 
   | tabs : ∀ Γ x x_ty e e_ty o,
             LExpr.fresh x e →
             (hx : LTy.isMonoType x_ty) →
             (he : LTy.isMonoType e_ty) →
-            HasType { Γ with types := Γ.types.insert x.fst x_ty} (LExpr.varOpen 0 x e) e_ty →
+            HasType C { Γ with types := Γ.types.insert x.fst x_ty} (LExpr.varOpen 0 x e) e_ty →
             o = none ∨ o = some (x_ty.toMonoType hx) →
-            HasType Γ (.abs o e)
+            HasType C Γ (.abs o e)
                       (.forAll [] (.tcons "arrow" [(LTy.toMonoType x_ty hx),
                                                    (LTy.toMonoType e_ty he)]))
 
   | tapp : ∀ Γ e1 e2 t1 t2,
             (h1 : LTy.isMonoType t1) →
             (h2 : LTy.isMonoType t2) →
-            HasType Γ e1 (.forAll [] (.tcons "arrow" [(LTy.toMonoType t2 h2),
+            HasType C Γ e1 (.forAll [] (.tcons "arrow" [(LTy.toMonoType t2 h2),
                                                      (LTy.toMonoType t1 h1)])) →
-            HasType Γ e2 t2 →
-            HasType Γ (.app e1 e2) t1
+            HasType C Γ e2 t2 →
+            HasType C Γ (.app e1 e2) t1
 
   -- `ty` is more general than `e_ty`, so we can instantiate `ty` with `e_ty`.
   | tinst : ∀ Γ e ty e_ty x x_ty,
-            HasType Γ e ty →
+            HasType C Γ e ty →
             e_ty = LTy.open x x_ty ty →
-            HasType Γ e e_ty
+            HasType C Γ e e_ty
 
   -- The generalization rule will let us do things like the following:
   -- `(·ftvar "a") → (.ftvar "a")` (or `a → a`) will be generalized to
   -- `(.btvar 0) → (.btvar 0)` (or `∀a. a → a`), assuming `a` is not in the
   -- context.
   | tgen : ∀ Γ e a ty,
-            HasType Γ e ty →
+            HasType C Γ e ty →
             TContext.isFresh a Γ →
-            HasType Γ e (LTy.close a ty)
+            HasType C Γ e (LTy.close a ty)
 
   | tif : ∀ Γ c e1 e2 ty,
-            HasType Γ c (.forAll [] .bool) →
-            HasType Γ e1 ty →
-            HasType Γ e2 ty →
-            HasType Γ (.ite c e1 e2) ty
+            HasType C Γ c (.forAll [] .bool) →
+            HasType C Γ e1 ty →
+            HasType C Γ e2 ty →
+            HasType C Γ (.ite c e1 e2) ty
 
   | teq : ∀ Γ e1 e2 ty,
-            HasType Γ e1 ty →
-            HasType Γ e2 ty →
-            HasType Γ (.eq e1 e2) (.forAll [] .bool)
+            HasType C Γ e1 ty →
+            HasType C Γ e2 ty →
+            HasType C Γ (.eq e1 e2) (.forAll [] .bool)
 
   | tquant: ∀ Γ k tr tr_ty x x_ty e o,
             LExpr.fresh x e →
             (hx : LTy.isMonoType x_ty) →
-            HasType { Γ with types := Γ.types.insert x.fst x_ty} (LExpr.varOpen 0 x e) (.forAll [] .bool) →
-            HasType {Γ with types := Γ.types.insert x.fst x_ty} (LExpr.varOpen 0 x tr) tr_ty →
+            HasType C { Γ with types := Γ.types.insert x.fst x_ty} (LExpr.varOpen 0 x e) (.forAll [] .bool) →
+            HasType C {Γ with types := Γ.types.insert x.fst x_ty} (LExpr.varOpen 0 x tr) tr_ty →
             o = none ∨ o = some (x_ty.toMonoType hx) →
-            HasType Γ (.quant k o tr e) (.forAll [] .bool)
+            HasType C Γ (.quant k o tr e) (.forAll [] .bool)
+  | top: ∀ Γ f op ty,
+            C.functions.find? (fun fn => fn.name == op) = some f →
+            f.type = .ok ty →
+            HasType C Γ (.op op none) ty
+  /-
+  See comments in `tvar_annotated`.
+  -/
+  | top_annotated: ∀ Γ f op ty_o ty_s tys,
+            C.functions.find? (fun fn => fn.name == op) = some f →
+            f.type = .ok ty_o →
+            tys.length = ty_o.boundVars.length →
+            LTy.openFull ty_o tys = ty_s →
+            HasType C Γ (.op op (some ty_s)) (.forAll [] ty_s)
 
 /--
 If `LExpr e` is well-typed, then it is well-formed, i.e., contains no dangling
 bound variables.
 -/
-theorem HasType.regularity (h : HasType (IDMeta:=IDMeta) Γ e ty) :
+theorem HasType.regularity (h : HasType (IDMeta:=IDMeta) C Γ e ty) :
   LExpr.WF e := by
   open LExpr in
   induction h <;> try (solve | simp_all[WF, lcAt])
@@ -148,45 +184,58 @@ section Tests
 
 open LExpr.SyntaxMono LTy.Syntax
 
-example : LExpr.HasType {} esM[#true] t[bool] := by
-  apply LExpr.HasType.tbool_const
+macro "solveKnownNames" : tactic =>  `(tactic | simp[KnownTypes.containsName, LTy.toKnownType!, makeKnownTypes, KnownTypes.default, LContext.default])
 
-example : LExpr.HasType {} esM[#-1] t[int] := by
-  apply LExpr.HasType.tint_const
+example : LExpr.HasType LContext.default {} esM[#true] t[bool] := by
+  apply LExpr.HasType.tbool_const; solveKnownNames
 
-example : LExpr.HasType { types := [[("x", t[∀a. %a])]]} esM[x] t[int] := by
-  have h_tinst := @LExpr.HasType.tinst (IDMeta := Unit) _ { types := [[("x", t[∀a. %a])]]} esM[x] t[∀a. %a] t[int] "a" mty[int]
-  have h_tvar := @LExpr.HasType.tvar (IDMeta := Unit) _ { types := [[("x", t[∀a. %a])]]} "x" t[∀a. %a]
-  simp +ground at h_tvar
-  simp [h_tvar] at h_tinst
-  simp +ground at h_tinst
-  exact h_tinst rfl
+example : LExpr.HasType LContext.default {} esM[#-1] t[int] := by
+  apply LExpr.HasType.tint_const; solveKnownNames
 
-example : LExpr.HasType { types := [[("m", t[∀a. %a → int])]]}
+example : LExpr.HasType LContext.default { types := [[("x", t[∀a. %a])]]} esM[x] t[int] := by
+  have h_tinst := @LExpr.HasType.tinst (IDMeta := Unit) _ LContext.default { types := [[("x", t[∀a. %a])]]} esM[x] t[∀a. %a] t[int] "a" mty[int]
+  have h_tvar := @LExpr.HasType.tvar (IDMeta := Unit) _ LContext.default { types := [[("x", t[∀a. %a])]]} "x" t[∀a. %a]
+  apply h_tinst; apply h_tvar; rfl
+  simp +ground; rfl
+
+example : LExpr.HasType LContext.default { types := [[("m", t[∀a. %a → int])]]}
                         esM[(m #true)]
                         t[int] := by
   apply LExpr.HasType.tapp _ _ _ _ t[bool] <;> (try simp +ground)
-  <;> try apply LExpr.HasType.tbool_const
+  <;> try apply LExpr.HasType.tbool_const <;> simp[KnownTypes.containsName]
   apply LExpr.HasType.tinst _ _ t[∀a. %a → int] t[bool → int] "a" mty[bool]
   · apply LExpr.HasType.tvar
     simp +ground
   · simp +ground
     exact rfl
+  solveKnownNames
   done
 
-example : LExpr.HasType {} esM[λ %0] t[∀a. %a → %a] := by
-  have h_tabs := @LExpr.HasType.tabs (IDMeta := Unit) _ {} ("a", none) t[%a] esM[%0] t[%a] none
-  simp +ground at h_tabs
-  have h_tvar := @LExpr.HasType.tvar (IDMeta := Unit) _ { types := [[("a", t[%a])]] }
+example : LExpr.HasType {} {} esM[λ %0] t[∀a. %a → %a] := by
+  have h_tabs := @LExpr.HasType.tabs (IDMeta := Unit) _ {} {} ("a", none) t[%a] esM[%0] t[%a] none
+  simp at h_tabs
+  have h_tvar := @LExpr.HasType.tvar (IDMeta := Unit) _ {} { types := [[("a", t[%a])]] }
                  "a" t[%a]
   simp [Maps.find?, Map.find?] at h_tvar
-  simp [h_tvar, LTy.toMonoType] at h_tabs
-  have h_tgen := @LExpr.HasType.tgen (IDMeta := Unit) _ {} esM[λ %0] "a"
+  specialize (h_tabs rfl rfl rfl h_tvar)
+  simp [LTy.toMonoType] at h_tabs
+  have h_tgen := @LExpr.HasType.tgen (IDMeta := Unit) _ {} {} esM[λ %0] "a"
                  t[%a → %a]
                  h_tabs
-  simp +ground [Maps.find?] at h_tgen
+  simp[TContext.isFresh, Maps.find?] at h_tgen
   assumption
   done
+
+def idFactory : LFunc Unit := {name := "id", typeArgs := ["a"],  inputs := [⟨"x", .ftvar "a"⟩], output := .ftvar "a"}
+
+example : LExpr.HasType (LContext.default.addFactoryFunction idFactory) {} (.op ⟨"id", ()⟩ none) t[∀a. %a → %a] := by
+  apply (LExpr.HasType.top _ idFactory) <;> rfl
+
+example : LExpr.HasType (LContext.default.addFactoryFunction idFactory) {} (.op ⟨"id", ()⟩ mty[int → int]) t[int → int] := by
+  apply (LExpr.HasType.top_annotated _ idFactory _ t[∀a. %a → %a] _ [.int]) <;> try rfl
+  simp only[LTy.openFull, LTy.toMonoTypeUnsafe, List.zip, LTy.boundVars];
+  unfold LMonoTy.subst ;
+  simp[Subst.hasEmptyScopes, Map.isEmpty, LMonoTys.subst, LMonoTys.subst.substAux, LMonoTy.subst, Maps.find?, Map.find?, LMonoTy.int]
 
 end Tests
 
